Append-only log done

composition/log.fst
@@ -3,13 +3,15 @@ open FStar.List.Tot
 
 open Library
 
-  val fst : e:(nat * string) -> Tot (id:nat {exists m. e = (id, m)})
-    let fst (id, m) = id
+val fst : e:(nat * string) -> Tot (id:nat {exists m. e = (id, m)})
+let fst (id, m) = id
 
-    val snd : e:(nat * string) -> Tot (m:string {exists id. e = (id, m)})
-    let snd (id, m) = m
-    
-val mem_id_s : id:nat -> l:list (nat * string) -> Tot (b:bool {b = true <==> (exists m. mem (id,m) l) /\ (exists e. mem e l ==> fst e = id)})
+val snd : e:(nat * string) -> Tot (m:string {exists id. e = (id, m)})
+let snd (id, m) = m
+
+val mem_id_s : id:nat 
+             -> l:list (nat * string) 
+             -> Tot (b:bool {b = true <==> (exists m. mem (id,m) l) /\ (exists e. mem e l ==> fst e = id)})
 let rec mem_id_s id l =
   match l with
   |[] -> false
@@ -21,44 +23,58 @@ let rec unique_s l =
   |[] -> true
   |(id,m)::xs -> not (mem_id_s id xs) && unique_s xs
 
- 
+val pos : id:(nat * string) 
+        -> l:list (nat * string) {mem id l /\ unique_s l} 
+        -> Tot nat
+let rec pos id l =
+  match l with
+  |id1::xs -> if id = id1 then 0 else 1 + pos id xs
 
-  val pos : id:(nat * string) -> l:list (nat * string) {mem id l /\ unique_s l} -> Tot nat
-    let rec pos id l =
-      match l with
-      |id1::xs -> if id = id1 then 0 else 1 + pos id xs
-
-val total_order : l:list (nat * string) {unique_s l}
-                -> Tot (b:bool)
+val total_order : l:list (nat * string) {unique_s l} -> Tot bool
 let rec total_order l =
   match l with
   |[] -> true
   |[x] -> true
-  |x::xs -> forallb (fun e -> fst x > fst e) xs && total_order xs
+  |x::xs ->  forallb (fun e -> fst x > fst e) xs && total_order xs
 
 val test_sorted: x:(nat * string) -> l:list (nat * string) ->
-                   Lemma ((unique_s (x::l) /\ total_order (x::l) /\ Cons? l) ==> fst x > fst (Cons?.hd l))
+                        Lemma ((unique_s (x::l) /\ total_order (x::l) /\ Cons? l) ==> fst x > fst (Cons?.hd l))
 let test_sorted x l = ()
 
 val ord : id:(nat * string)
-            -> id1:(nat * string)
-            -> l:list (nat * string)
-            -> Pure bool
-              (requires fst id <> fst id1 /\ mem id l /\ mem id1 l /\ unique_s l /\ total_order l)
-              (ensures (fun b -> b = true <==> pos id l < pos id1 l))
+        -> id1:(nat * string) {fst id <> fst id1}
+        -> l:list (nat * string) {mem id l /\ mem id1 l /\ unique_s l /\ total_order l}
+        -> Tot (b:bool {b = true <==> pos id l < pos id1 l})
 let ord id id1 l = pos id l < pos id1 l 
 
 val sorted_smaller: x:(nat * string)
-                      ->  y:(nat * string)
-                      ->  l:list (nat * string)
-                      ->  Lemma (requires (unique_s (x::l) /\ total_order (x::l) /\ mem y l))
-                                (ensures (fst x > fst y) /\ ord x y (x::l))
-                                [SMTPat (unique_s (x::l) /\ total_order (x::l))]
+                  ->  y:(nat * string)
+                  ->  l:list (nat * string)
+                  ->  Lemma (requires (unique_s (x::l) /\ total_order (x::l) /\ mem y l))
+                           (ensures (fst x > fst y) /\ ord x y (x::l))
+                                    [SMTPat (unique_s (x::l) /\ total_order (x::l))]
+
+#set-options "--z3rlimit 1000000"
 let rec sorted_smaller x y l = match l with
-      | [] -> ()
-      | z::zs -> if z=y then () else sorted_smaller x y zs
-      
+          | [] -> ()
+          | z::zs -> if z=y then () else sorted_smaller x y zs
+
 type s = l: list (nat (*id*) * string (*message*)) {unique_s l /\ total_order l}
+
+val filter_uni : f:((nat * string) -> bool)
+               -> l:list (nat * string) 
+               -> Lemma (requires (unique_s l /\ total_order l))
+                       (ensures (unique_s (filter f l) /\ total_order (filter f l)) /\
+                                 (forall e. mem e l /\ f e <==> mem e (filter f l)) /\
+                          (forall e e1. mem e l /\ mem e1 l /\ f e /\ f e1 /\ fst e <> fst e1 /\ fst e > fst e1 /\ ord e e1 l <==>
+       mem e (filter f l) /\ mem e1 (filter f l) /\ fst e <> fst e1 /\ fst e > fst e1 /\ ord e e1 (filter f l)))
+                               [SMTPat (filter f l)]
+
+#set-options "--z3rlimit 1000000"
+let rec filter_uni f l =
+  match l with
+  |[] -> ()
+  |x::xs -> filter_uni f xs
 
 type op =
   |Append : string (*message*) -> op
@@ -68,7 +84,6 @@ let get_msg (id, (Append m)) = m
 
 val get_id : op1:(nat * op) -> Tot (id:nat {exists m. op1 = (id, (Append m))}) 
 let get_id (id, (Append m)) = id
-
 
 val app_op : s1:s 
            -> op1:(nat * op)
@@ -81,52 +96,43 @@ val app_op : s1:s
 #set-options "--z3rlimit 1000000"
 let app_op s1 (id, (Append m)) = (id, m)::s1
 
-val filter_uni : f:((nat * string) -> bool)
-                 -> l:list (nat * string) 
-                 -> Lemma (requires (unique_s l /\ total_order l))
-                          (ensures (unique_s (filter f l) /\ total_order (filter f l)) /\
-                            (forall e. mem e l /\ f e <==> mem e (filter f l)) /\
-                            (forall e e1. mem e l /\ mem e1 l /\ fst e <> fst e1 /\ fst e > fst e1 /\ ord e e1 l /\ f e /\ f e1 <==>
-                     mem e (filter f l) /\ mem e1 (filter f l) /\ fst e <> fst e1 /\ fst e > fst e1 /\ ord e e1 (filter f l)))
-                          [SMTPat (filter f l)]
-
-#set-options "--z3rlimit 1000000"
-let rec filter_uni f l =
-    match l with
-    |[] -> ()
-    |x::xs -> filter_uni f xs
-
 val filter_uni1 : f:((nat * op) -> bool)
-                   -> l:list (nat * op) 
-                   -> Lemma (requires (unique l))
-                           (ensures (unique (filter f l)))
+                -> l:list (nat * op) 
+                -> Lemma (requires (unique l))
+                        (ensures (unique (filter f l)))
                            [SMTPat (filter f l)]
 let rec filter_uni1 f l = 
-      match l with
-      |[] -> ()
-      |x::xs -> filter_uni1 f xs
-      
+  match l with
+  |[] -> ()
+  |x::xs -> filter_uni1 f xs
+
 (*)instance log : datatype s op = {
   Library.app_op = app_op
 }*)
+
+val filter_s : f:((nat * string) -> bool)
+             -> l:s
+             -> Tot (l1:s {forall e. mem e l1 <==> mem e l /\ f e})
+let rec filter_s  f l = 
+          match l with
+          |[] -> []
+          |hd::tl -> if f hd then hd::(filter_s f tl) else filter_s f tl
 
 #set-options "--query_stats"
 val sim : tr:ae op
         -> s1:s
         -> Tot (b:bool {b = true <==> (forall e. mem e s1 <==> mem (fst e, (Append (snd e))) tr.l) /\
-                                   (forall e e1. mem e s1 /\ mem e1 s1 /\ fst e <> fst e1 /\ fst e > fst e1 /\ ord e e1 s1 <==>
-                                      (mem (fst e, (Append (snd e))) tr.l /\ mem (fst e1, (Append (snd e1))) tr.l /\
-               fst e <> fst e1 /\ fst e > fst e1 (*)/\ (tr.vis (fst e1, (Append (snd e1))) (fst e, (Append (snd e))) \/
-               not (tr.vis (fst e1, (Append (snd e1))) (fst e, (Append (snd e))) ||
-               tr.vis (fst e, (Append (snd e))) (fst e1, (Append (snd e1))))*)))})
+                                     (forall e e1. (mem (fst e, (Append (snd e))) tr.l /\ 
+                                          mem (fst e1, (Append (snd e1))) tr.l /\ fst e <> fst e1 /\ fst e > fst e1) <==>
+                                          mem e s1 /\ mem e1 s1 /\ fst e <> fst e1 /\ fst e > fst e1 /\ ord e e1 s1)})
 
 #set-options "--z3rlimit 1000000"
 let sim tr s1 = 
   forallb (fun e -> mem (fst e, (Append (snd e))) tr.l) s1 &&
   forallb (fun e -> mem (get_id e, get_msg e) s1) tr.l &&
   forallb (fun e -> (forallb (fun e1 -> (mem (fst e, (Append (snd e))) tr.l && mem (fst e1, (Append (snd e1))) tr.l &&
-              fst e <> fst e1 && fst e > fst e1)) 
-  (filter (fun e1 -> mem e1 s1 && mem e s1 && fst e <> fst e1 && fst e > fst e1 && ord e e1 s1) s1))) s1 &&
+              fst e <> fst e1 && fst e > fst e1))
+  (filter_s (fun e1 -> mem e1 s1 && mem e s1 && fst e <> fst e1 && fst e > fst e1 && ord e e1 s1) s1))) s1 &&
   forallb (fun e -> (forallb (fun e1 -> mem (get_id e, get_msg e) s1 && mem (get_id e1, get_msg e1) s1 && get_id e <> get_id e1 && get_id e > get_id e1 && ord (get_id e, get_msg e) (get_id e1, get_msg e1) s1)
           (filter (fun e1 -> (get_id e <> get_id e1 && get_id e > get_id e1)) tr.l))) tr.l
 
@@ -143,76 +149,42 @@ let prop_oper tr st op = ()
 val remove_st : ele:(nat * string) -> a:s
                   -> Pure s
                     (requires (mem ele a))
-                    (ensures (fun r -> (forall e. mem e r <==> mem e a /\ e <> ele) (*)/\
-                                    (forall id. mem_id_s id r <==> mem_id_s id a /\ id <> fst ele*) /\
+                    (ensures (fun r -> (forall e. mem e r <==> mem e a /\ e <> ele) /\
                                     (forall e e1. mem e r /\ mem e1 r /\ fst e <> fst e1 /\ ord e e1 r /\ fst e > fst e1 <==>
-                         mem e a /\ mem e1 a /\ fst e <> fst e1 /\ e <> ele /\ e1 <> ele /\ fst e > fst e1 /\ ord e e1 a) (*)/\
-                                            List.Tot.length r = List.Tot.length a - 1*) ))
+                         mem e a /\ mem e1 a /\ fst e <> fst e1 /\ e <> ele /\ e1 <> ele /\ fst e > fst e1 /\ ord e e1 a)))
 
 #set-options "--z3rlimit 1000000"
-let rec remove_st ele a = filter (fun e -> e <> ele) a
+let remove_st ele a = filter (fun e -> e <> ele) a
 
 val convergence : tr:ae op
-                    -> a:s
-                    -> b:s
-                    -> Lemma (requires (sim tr a /\ sim tr b))
-                            (ensures (forall id. mem_id_s id a <==> mem_id_s id b) /\ (forall e. mem e a <==> mem e b) /\
-                                     (forall e e1. mem e a /\ mem e1 a /\ fst e <> fst e1 /\ ord e e1 a /\ fst e > fst e1 <==> 
-                                              mem e b /\ mem e1 b /\ fst e <> fst e1 /\ ord e e1 b /\ fst e > fst e1))
-                            (*)[SMTPat (sim tr a /\ sim tr b)]*)
+                -> a:s
+                -> b:s
+                -> Lemma (requires (sim tr a /\ sim tr b))
+                        (ensures (forall id. mem_id_s id a <==> mem_id_s id b) /\ (forall e. mem e a <==> mem e b) /\
+                                 (forall e e1. mem e a /\ mem e1 a /\ fst e <> fst e1 /\ ord e e1 a /\ fst e > fst e1 <==> 
+                                          mem e b /\ mem e1 b /\ fst e <> fst e1 /\ ord e e1 b /\ fst e > fst e1))
 let convergence tr a b = ()
 
-(*)val help : a:s 
-         -> Lemma (ensures (forall e e1. mem e a /\ mem e1 a /\ fst e <> fst e1 /\ fst e > fst e1 ==>
-                                   fst e <> fst e1 /\ mem e a /\ mem e1 a /\ ord e e1 a))
-                                   [SMTPat (unique_s a /\ total_order a)]
+val union_s : a:s
+            -> b:s
+            -> Pure s
+                 (requires (forall e. mem e a ==> not (mem_id_s (fst e) b)) /\ 
+                           (forall e. mem e b ==> not (mem_id_s (fst e) a)))
+                   (ensures (fun u -> (forall e. mem e u <==> mem e a \/ mem e b)/\
+                                 (forall e e1. ((mem e a /\ mem e1 a /\ fst e <> fst e1 /\ fst e > fst e1 /\ ord e e1 a) \/
+                                 (mem e b /\ mem e1 b /\ fst e <> fst e1 /\ fst e > fst e1 /\ ord e e1 b) \/
+                                 (mem e a /\ mem e1 b /\ fst e <> fst e1 /\ fst e > fst e1) \/
+                                 (mem e b /\ mem e1 a /\ fst e <> fst e1 /\ fst e > fst e1)) <==>
+                                 (mem e u /\ mem e1 u /\ fst e <> fst e1 /\ fst e > fst e1 /\ ord e e1 u))))
 
 #set-options "--z3rlimit 10000000"
-let rec help a = admit ();
-  match a with
-  |[] -> ()
-  |x::xs -> help xs*)
-
-
-val merge1 : l:s -> a:s -> b:s
-           -> Pure s
-             (requires (forall e. mem e l ==> mem e a /\ mem e b) /\
-                       (forall e e1. mem e a /\ not (mem e l) /\ mem e1 b /\ not (mem e1 l) ==> e <> e1))
-             (ensures (fun r -> (forall e. mem e r <==> mem e a \/ mem e b) /\
-                             (forall e e1. mem e r /\ mem e1 r /\ fst e <> fst e1 /\ fst e > fst e1 /\ ord e e1 r <==>
-                                     (mem e a /\ mem e1 a /\ fst e <> fst e1 /\ fst e > fst e1 /\ ord e e1 a) \/
-                                     (mem e b /\ mem e1 b /\ fst e <> fst e1 /\ fst e > fst e1 /\ ord e e1 b) \/
-                                     (mem e a /\ mem e1 b /\ fst e <> fst e1 /\ fst e > fst e1) \/
-                                     (mem e b /\ mem e1 a /\ fst e <> fst e1 /\ fst e > fst e1))))
-                                     (decreases %[l;a;b])
-
-#set-options "--z3rlimit 10000000"
-let rec merge1 l a b = admit()
-
-val un : a:s -> b:s
-       -> Pure s
-         (requires (forall id. mem_id_s id a ==> not (mem_id_s id b)) /\
-                   (forall e e1. mem e a /\ mem e1 b ==> fst e <> fst e1))
-         (ensures (fun r -> (forall e. mem e r <==> mem e a \/ mem e b) /\
-                         (forall e e1. 
-                                      (mem e a /\ mem e1 a /\ fst e <> fst e1 /\ fst e > fst e1 /\ ord e e1 a) \/
-                                      (mem e b /\ mem e1 b /\ fst e <> fst e1 /\ fst e > fst e1 /\ ord e e1 b) \/
-                                      (mem e a /\ mem e1 b /\ fst e <> fst e1 /\ fst e > fst e1) \/
-                                      (mem e b /\ mem e1 a /\ fst e <> fst e1 /\ fst e > fst e1) ==>
-                                      mem e r /\ mem e1 r /\ fst e <> fst e1 /\ fst e > fst e1 /\ ord e e1 r)))
-
-#set-options "--z3rlimit 1000000"
-let rec un a b =
-  match a, b with
-  |[],[] -> []
-  |[],_ -> b
-  |x::xs,[] -> a 
-  |x::xs, y::ys -> if fst x > fst y then 
-                ((*)assume (forall e e1. mem e xs /\ mem e1 b ==> fst x > fst e /\ fst x > fst e1 /\ ord x e (x::(un xs b)) /\ 
-                        ord x e1 (x::(un xs b)));*)
-                       admit (); x::(un xs b)) else 
-                ((*)assume (forall e e1. mem e ys /\ mem e1 a ==> fst y > fst e /\ fst y > fst e1 /\ ord y e (y::(un a ys)) /\ 
-                         ord y e1 (y::(un a ys)));*)admit(); y::(un a ys))
+let rec union_s l1 l2 =
+    match l1, l2 with
+    | [], [] -> []
+    | [], l2 -> l2
+    | l1, [] -> l1
+    | h1::t1, h2::t2 -> if (fst h1 > fst h2)
+                     then h1::(union_s t1 l2) else h2::(union_s l1 t2)
 
 val merge : ltr:ae op
           -> l:s
@@ -231,15 +203,7 @@ val merge : ltr:ae op
                                         (mem e a /\ mem e1 a /\ fst e <> fst e1 /\ fst e > fst e1 /\ ord e e1 a) \/
                                         (mem e b /\ mem e1 b /\ fst e <> fst e1 /\ fst e > fst e1 /\ ord e e1 b) \/
                                         (mem e a /\ mem e1 b /\ fst e <> fst e1 /\ fst e > fst e1) \/
-                                        (mem e b /\ mem e1 a /\ fst e <> fst e1 /\ fst e > fst e1))
-                               (*forall e e1. mem e r /\ mem e1 r /\ fst e <> fst e1 /\ fst e > fst e1 /\ ord e e1 r <==>
-                            (mem e l /\ mem e1 l /\ fst e <> fst e1 /\ fst e > fst e1 /\ ord e e1 l) \/
-                            (mem e (diff a l) /\ mem e1 (diff a l) /\ fst e <> fst e1 /\ fst e > fst e1 /\ ord e e1 (diff a l)) \/
-                            (mem e (diff b l) /\ mem e1 (diff b l) /\ fst e <> fst e1 /\ fst e > fst e1 /\ ord e e1 (diff b l)) \/
-                            (mem e (diff a l) /\ mem e1 l /\ fst e <> fst e1 /\ fst e > fst e1) \/
-                            (mem e (diff b l) /\ mem e1 l /\ fst e <> fst e1 /\ fst e > fst e1) \/
-                            (mem e (diff a l) /\ mem e1 (diff b l) /\ fst e <> fst e1 /\ fst e > fst e1) \/
-                            (mem e (diff b l) /\ mem e1 (diff a l) /\ fst e <> fst e1 /\ fst e > fst e1)*)))
+                                        (mem e b /\ mem e1 a /\ fst e <> fst e1 /\ fst e > fst e1))))
 
 #set-options "--z3rlimit 10000000"
 let merge ltr l atr a btr b = 
@@ -252,10 +216,10 @@ let merge ltr l atr a btr b =
   assert (unique_s lb /\ total_order lb);
   assert (forall e e1. mem e l /\ mem e1 lb ==> fst e1 > fst e);
   assert (forall id. mem_id_s id la ==> not (mem_id_s id lb));
-  let u = un la lb in
+  let u = union_s la lb in
   assert (forall id. mem_id_s id l ==> not (mem_id_s id u));
   assert (forall e e1. mem e l /\ mem e1 u ==> fst e <> fst e1);
-  un u l
+  union_s u l
 
 val prop_merge : ltr:ae op
                -> l:s
@@ -273,23 +237,17 @@ val prop_merge : ltr:ae op
 
 #set-options "--z3rlimit 10000000"
 let prop_merge ltr l atr a btr b = 
-  (*)lem_abs ltr atr btr;*)
     assert (forall e. mem e (merge ltr l atr a btr b) <==> mem (fst e, (Append (snd e))) (absmerge ltr atr btr).l);
     assert (forall e e1. mem e (merge ltr l atr a btr b) /\ mem e1 (merge ltr l atr a btr b) /\ fst e <> fst e1 /\ 
                 fst e > fst e1 /\ ord e e1 (merge ltr l atr a btr b) ==>
                 mem (fst e, (Append (snd e))) (absmerge ltr atr btr).l /\ 
                 mem (fst e1, (Append (snd e1))) (absmerge ltr atr btr).l /\
-                fst e <> fst e1 /\ fst e > fst e1 (*)/\ 
-                ((absmerge ltr atr btr).vis (fst e1, (Append (snd e1))) (fst e, (Append (snd e))) \/
-                  not ((absmerge ltr atr btr).vis (fst e1, (Append (snd e1))) (fst e, (Append (snd e))) ||
-                    (absmerge ltr atr btr).vis (fst e, (Append (snd e))) (fst e1, (Append (snd e1))))*));
+                fst e <> fst e1 /\ fst e > fst e1);
     assert (forall e e1. mem e (absmerge ltr atr btr).l /\ mem e1 (absmerge ltr atr btr).l /\ get_id e <> get_id e1 /\ 
-                    get_id e > get_id e1 (*)/\ ((absmerge ltr atr btr).vis e1 e \/
-                           not ((absmerge ltr atr btr).vis e e1 || (absmerge ltr atr btr).vis e1 e)*) ==> 
-                      mem (get_id e, get_msg e) (merge ltr l atr a btr b) /\ 
+                    get_id e > get_id e1 ==> mem (get_id e, get_msg e) (merge ltr l atr a btr b) /\ 
                         mem (get_id e1, get_msg e1) (merge ltr l atr a btr b) /\
              get_id e <> get_id e1 /\ get_id e > get_id e1 /\ 
-             ord (get_id e, get_msg e) (get_id e1, get_msg e1) (merge ltr l atr a btr b)); (*done*)
+             ord (get_id e, get_msg e) (get_id e1, get_msg e1) (merge ltr l atr a btr b));
     ()
 
 (*)instance _ : mrdt s op log = {
